Proof is failing, back to the drawing board...

src/fs/Interpreter.fs
@@ -21,7 +21,7 @@ type interpretation<'state> =
   { alloc      : 'state -> BoolExp -> (int * 'state);
     assign     : 'state -> int -> BoolExp -> 'state;
     clean      : 'state -> GExpr -> int -> 'state;
-    apply      : 'state -> 'state -> GExpr -> 'state;
+    (*apply      : 'state -> 'state -> GExpr -> 'state;*)
     assertion  : 'state -> GExpr -> int -> 'state;
     eval       : 'state -> Total.state -> int -> bool }
 
@@ -188,9 +188,10 @@ let rec eval_rec (tm, st) interp = match tm with
     bind (eval_rec (t1, st) interp)  (fun (v1, st') ->
     bind (eval_rec (t2, st') interp) (fun (v2, st'') ->
     begin match v1 with
-      | LAMBDA (x, ty, t) -> 
+      | LAMBDA (x, ty, t) -> eval_rec (substGExpr t x v2, st'') interp 
+          (*
           bind (eval_rec (substGExpr t x v2, st'') interp) (fun (v, st''') ->
-            Val (v, interp.apply st'' st''' (APPLY (v1, v2))))
+            Val (v, interp.apply st'' st''' (APPLY (v1, v2))))*)
       | _ -> Err ("LHS is not a lambda: " ^ (show tm))
     end))
   | SEQUENCE (t1, t2) ->
@@ -302,7 +303,7 @@ let boolEval (top, st) ivals i = lookup st i
 let boolInterp = {
   alloc = boolAlloc;
   assign = boolAssign;
-  apply = fun st st' t -> st'
+  (*apply = fun st st' t -> st'*)
   clean = fun st t l -> st;
   assertion = fun st t l -> st;
   eval = boolEval
@@ -336,7 +337,7 @@ let bexpEval (top, st) ivals i = evalBexp (lookup st i) ivals
 let bexpInterp = {
   alloc = bexpAlloc;
   assign = bexpAssign;
-  apply = fun st st' t -> st'
+  (*apply = fun st st' t -> st'*)
   clean = fun st t l -> st;
   assertion = fun st t l -> st;
   eval = bexpEval
@@ -471,7 +472,7 @@ let circEval (top, ah, circ, st, cl) ivals i = lookup (evalCirc circ ivals) (loo
 let circInterp = {
   alloc = circAlloc;
   assign = circAssign;
-  apply = fun st st' t -> st'
+  (*apply = fun st st' t -> st'*)
   clean = circClean;
   assertion = fun st t l -> st;
   eval = circEval
@@ -606,19 +607,19 @@ let circGCClean cs _ l =
     { top = cs.top; ah = insert cs.ah bit.id; gates = cs.gates; symtab = Partial.update cs.symtab l q' }
 let circGCEval cs st i = false
 
-(* For uncoupling dependencies with constant assertions *)
+(* For uncoupling dependencies with constant assertions
 let circGCApply st st' t = match t with
   | APPLY (LAMBDA (x, ty, t), v) ->
       let modSet = getMods (substGExpr t x v, st) in
       let rem
         begin match ty with
           | GConst 
-  | _ -> st'
+  | _ -> st'*)
 
 let circGCInterp = {
   alloc = circGCAlloc;
   assign = circGCAssign;
-  apply = fun st st' t -> st'
+  (*apply = fun st st' t -> st'*)
   clean = circGCClean;
   assertion = fun st t l -> st;
   eval = circGCEval
