src/GC.fst
@@ -16,21 +16,24 @@ type qubit =
     ival : BoolExp;
     cval : BoolExp }
 
-val null_q : qubit
-val get_subst : Partial.t int qubit -> int -> Tot int
-val data_q : int -> Tot qubit
-val anc_q  : int -> Tot qubit
+val null_q  : qubit
+val getSubs : Total.t int qubit -> Tot (Total.t int int)
+val ids     : Total.t int qubit -> Tot (set int)
+val data_q  : int -> Tot qubit
+val anc_q   : int -> Tot qubit
 
-let nullq = { id = 0; ival = BFalse; cval = BFalse }
-let get_subst m = fun i -> (Partial.find_def m i nullq).id
+let nullq    = { id = 0; ival = BFalse; cval = BFalse }
+let getSubs  = mapVals (fun q -> q.id)
+let ids m    = vals (getSubs m)
 let data_q i = { id = i; ival = BVar i; cval = BFalse }
 let anc_q i  = { id = i; ival = BFalse; cval = BFalse }
+
 
 type circGCState =
   { top    : int;
     ah     : AncHeap;
     gates  : list Gate;
-    symtab : Partial.t int qubit }
+    symtab : Total.t int qubit }
 
 val circGC       : circGCState -> int -> Tot circGCState
 val circGCInit   : circGCState
@@ -50,9 +53,9 @@ let garbageCollect cs q =
     let subq = fun v -> if v = q.id then BXor (q.ival, q.cval) else BVar v in
       { id   = q'.id; 
         ival = q'.ival; 
-	cval = simplify (substBexpf q'.cval subq) }
+	cval = substBexpf q'.cval subq }
   in
-  let symtab' = Partial.mapVals f cs.symtab in
+  let symtab' = mapVals f cs.symtab in
     { top    = cs.top; 
       ah     = ah''; 
       gates  = cs.gates @ circ; 
@@ -62,10 +65,10 @@ let circGCInit =
   { top    = 0; 
     ah     = emptyHeap; 
     gates  = []; 
-    symtab = [] }
+    symtab = constMap nullq }
 
 let circGCAlloc cs bexp = 
-  let bexp' = simplify (substVarf bexp (get_subst cs.symtab)) in
+  let bexp' = substVar bexp (getSubs cs.symtab) in
   let (ah', bit) = popMin cs.ah in
   let (ah'', res, ancs, circ') = compileBexp ah' bit bexp' in
   let q = { id = bit; 
@@ -74,12 +77,12 @@ let circGCAlloc cs bexp =
   in
   let top' = cs.top + 1 in
   let gates' = cs.gates @ circ' in
-  let symtab' = Partial.update cs.symtab cs.top q in
-  (cs.top, {top = top'; ah = ah''; gates = gates'; symtab = symtab'})
+  let symtab' = update cs.symtab cs.top q in
+    (cs.top, {top = top'; ah = ah''; gates = gates'; symtab = symtab'})
 
 let circGCAssign cs l bexp =
-  let q = Partial.find_def cs.symtab l nullq in
-  let bexp' = simplify (substVarf bexp (get_subst cs.symtab)) in
+  let q = lookup cs.symtab l in
+  let bexp' = substVar bexp (getSubs cs.symtab) in
   let bexpfac = factorAs bexp' q.id in
   match (q.cval, bexpfac) with
     | (BFalse, _)      -> // substitute q.id with BFalse, compile in place
@@ -90,23 +93,23 @@ let circGCAssign cs l bexp =
 	let subq = fun v -> if v = q.id then bexp'' else BVar v in
 	  { id = b.id; 
 	    ival = b.ival; 
-	    cval = simplify (substBexpf b.cval subq) }
+	    cval = substBexpf b.cval subq }
       in
-      let symtab' = Partial.update (Partial.mapVals f cs.symtab) l q' in
+      let symtab' = update (mapVals f cs.symtab) l q' in
         { top = cs.top; 
 	  ah = ah'; 
 	  gates = cs.gates @ circ; 
 	  symtab = symtab' }
     | (_, Some bexp'') -> // compile in place, substitute q.id with q.id \oplus bexp''
       let (ah', res, ancs, circ') = compileBexp cs.ah q.id bexp'' in
-      let q' = { id = q.id; ival = q.ival; cval = simplify (BXor (q.cval, bexp'')) } in
+      let q' = { id = q.id; ival = q.ival; cval = BXor (q.cval, bexp'') } in
       let f b = 
         let subq = fun v -> if v = q.id then BXor (BVar q.id, bexp'') else BVar v in
 	  { id = b.id; 
 	    ival = b.ival; 
-	    cval = simplify (substBexpf b.cval subq) }
+	    cval = substBexpf b.cval subq }
       in
-      let symtab' = Partial.update (Partial.mapVals f cs.symtab) l q' in
+      let symtab' = update (mapVals f cs.symtab) l q' in
         { top = cs.top; 
 	  ah = ah'; 
 	  gates = cs.gates @ circ'; 
@@ -118,11 +121,11 @@ let circGCAssign cs l bexp =
 	{ top = cs.top; 
 	  ah = ah'; 
 	  gates = cs.gates @ circ'; 
-	  symtab = Partial.update cs.symtab l q' } 
+	  symtab = update cs.symtab l q' } 
       in
         garbageCollect cs' q
 
-let circGCEval cs st i = false
+let circGCEval cs st i = lookup (evalCirc cs.gates st) (lookup cs.symtab i).id
 
 let circGCInterp = {
   alloc = circGCAlloc;
@@ -139,7 +142,7 @@ let rec allocNcircGC (locs, cs) i =
     let cs' = { top = cs.top + 1;
                 ah = ah';
                 gates = cs.gates;
-                symtab = Partial.update cs.symtab cs.top (data_q res) }
+                symtab = update cs.symtab cs.top (data_q res) }
     in
       allocNcircGC (((LOC cs.top)::locs), cs') (i-1)
 
@@ -150,7 +153,7 @@ let allocTycircGC ty cs = match ty with
     let cs' = { top = cs.top + 1;
                 ah = ah';
                 gates = cs.gates;
-                symtab = Partial.update cs.symtab cs.top (data_q res) }
+                symtab = update cs.symtab cs.top (data_q res) }
     in
       Val (LOC cs.top, cs')
   | GArray n ->
@@ -158,26 +161,26 @@ let allocTycircGC ty cs = match ty with
       Val (ARRAY locs, st')
   | _ -> Err "Invalid parameter type for circuit generation"
 
-val lookup_Lst_gc : Partial.t int qubit -> lst:(list GExpr){isVal_lst lst} -> Tot (list int)
+val lookup_Lst_gc : Total.t int qubit -> lst:(list GExpr){isVal_lst lst} -> Tot (list int)
 let rec lookup_Lst_gc symtab lst = match lst with
   | [] -> []
-  | (LOC l)::xs -> ((Partial.find_def symtab l nullq).id)::(lookup_Lst_gc symtab xs)
+  | (LOC l)::xs -> ((lookup symtab l).id)::(lookup_Lst_gc symtab xs)
 
-(* Scrubs the state with respect to the remainder of the program *)
-let findGarbage gexp cs = Set.diff (Partial.keys cs.symtab) (locs gexp)
+(* Scrubs the state with respect to the remainder of the program
+let findGarbage gexp cs = Set.diff (keys cs.symtab) (locs gexp)
 let garbageCollector gexp cs = 
   let garbage = findGarbage gexp cs in
   let f cs l = 
-    let q = Partial.find_def cs.symtab l nullq in
+    let q = lookup cs.symtab l in
     let cs' = garbageCollect cs q in
-    { top = cs'.top; ah = cs'.ah; gates = cs'.gates; symtab = Partial.remove cs'.symtab l }
+    { top = cs'.top; ah = cs'.ah; gates = cs'.gates; symtab = remove cs'.symtab l }
   in
     cs
-  //Set.fold f cs garbage
+  //Set.fold f cs garbage *)
 
 val compileGCCirc : config circGCState -> Dv (result (list int * list Gate))
 let rec compileGCCirc (gexp, cs) =
-  let cs = garbageCollector gexp cs in
+  let cs = cs in //garbageCollector gexp cs in
   if isVal gexp then match gexp with
     | UNIT -> Val ([], [])
     | LAMBDA (x, ty, t) ->
@@ -186,7 +189,7 @@ let rec compileGCCirc (gexp, cs) =
         | Val (v, cs') -> compileGCCirc (substGExpr t x v, cs')
       end
     | LOC l ->
-      let res = Partial.find_def cs.symtab l nullq in
+      let res = lookup cs.symtab l in
         Val ([res.id], cs.gates)
     | ARRAY lst ->
       let res = lookup_Lst_gc cs.symtab lst in
@@ -195,3 +198,158 @@ let rec compileGCCirc (gexp, cs) =
     | Err s -> Err s
     | Val c' -> compileGCCirc c'
 
+(** Verification utilities *)
+
+(* A GCstate is valid w.r.t a set of initial values if
+     - the heap starts above 0
+     - everything on the heap is 0-valued after executing the circuit
+     - no active qubit is in the heap
+     - for every active qubit, q.ival = q' <> q.cval' *)
+type validGCState (cs:circGCState) (init:state) =
+  zeroHeap (evalCirc cs.gates init) cs.ah /\ 
+  disjoint (ids cs.symtab) (elts cs.ah) /\
+  (forall q. Set.mem q (vals cs.symtab) ==> 
+    evalBexp q.ival init = evalBexp (BXor (BVar q.id, q.cval)) (evalCirc cs.gates init))
+
+val subst_subset_active : cs:circGCState -> bexp:BoolExp ->
+  Lemma (subset (vars (substVar bexp (getSubs cs.symtab))) (ids cs.symtab))
+  (decreases bexp)
+let rec subst_subset_active cs bexp = match bexp with
+  | BFalse -> ()
+  | BVar i -> admit() //lookup_is_val cs.symtab i -- no reason this should fail
+  | BNot x -> subst_subset_active cs x
+  | BAnd (x, y) | BXor (x, y) -> 
+    subst_subset_active cs x;
+    subst_subset_active cs y
+
+(* These proofs are too big, takes forever to develop *)
+val valid_alloc1 : cs:circGCState -> init:state -> bexp:BoolExp -> cs':circGCState ->
+  Lemma (requires (validGCState cs init /\ cs' = snd (circGCAlloc cs bexp)))
+	(ensures  (zeroHeap (evalCirc cs'.gates init) cs'.ah))
+let valid_alloc1 cs init bexp cs' =
+  let bexp' = substVar bexp (getSubs cs.symtab) in
+  let (ah, bit) = popMin cs.ah in
+  let (ah', _, _, gates) = compileBexp ah bit bexp' in
+  let q = { id = bit; 
+            ival = BFalse; 
+            cval = bexp' } 
+  in
+  let init' = evalCirc cs'.gates init in
+    pop_proper_subset cs.ah;
+    zeroHeap_subset (evalCirc cs.gates init) cs.ah ah;
+    compile_decreases_heap ah bit bexp';
+    zeroHeap_subset (evalCirc cs.gates init) ah cs'.ah;
+    //------------
+    subst_subset_active cs bexp;
+    disjoint_subset (elts ah) (elts cs.ah) (ids cs.symtab);
+    disjoint_subset (vars bexp') (ids cs.symtab) (elts ah);
+    compile_partition ah bit bexp';
+    zeroHeap_st_impl (evalCirc cs.gates init) cs'.ah gates
+
+val valid_alloc2 : cs:circGCState -> init:state -> bexp:BoolExp -> cs':circGCState ->
+  Lemma (requires (validGCState cs init /\ cs' = snd (circGCAlloc cs bexp)))
+	(ensures  (disjoint (ids cs'.symtab) (elts cs'.ah)))
+let valid_alloc2 cs init bexp cs' =
+  let bexp' = substVar bexp (getSubs cs.symtab) in
+  let (ah, bit) = popMin cs.ah in
+  let (ah', _, _, gates) = compileBexp ah bit bexp' in
+  let q = { id = bit; 
+            ival = BFalse; 
+            cval = bexp' } 
+  in
+  let init' = evalCirc cs'.gates init in
+    pop_proper_subset cs.ah;
+    compile_decreases_heap ah bit bexp'
+
+val valid_alloc4 : cs:circGCState -> init:state -> bexp:BoolExp -> cs':circGCState -> bit:int ->
+  Lemma (requires (validGCState cs init /\ cs' = snd (circGCAlloc cs bexp)))
+        (ensures  (evalBexp BFalse init = evalBexp (BXor (BVar (get_min cs.ah), 
+	                                                  (substVar bexp (getSubs cs.symtab))))
+	                                           (evalCirc cs'.gates init)))
+let valid_alloc4 cs init bexp cs' bit =
+  let bexp' = substVar bexp (getSubs cs.symtab) in
+  let (ah, bit) = popMin cs.ah in
+  let (ah', _, _, gates) = compileBexp ah bit bexp' in
+  let q = { id = bit; 
+            ival = BFalse; 
+            cval = bexp' } 
+  in
+  let init' = evalCirc cs'.gates init in
+    pop_proper_subset cs.ah;
+    zeroHeap_subset (evalCirc cs.gates init) cs.ah ah;
+    //------------
+    subst_subset_active cs bexp;
+    disjoint_subset (elts ah) (elts cs.ah) (ids cs.symtab);
+    disjoint_subset (vars bexp') (ids cs.symtab) (elts ah);
+    //------------
+    compile_bexp_correct ah bit bexp' (evalCirc cs.gates init);
+    eval_mod (evalCirc cs.gates init) gates;
+    eval_state_swap (BXor (BVar q.id, q.cval)) (evalCirc cs.gates init) init'
+
+val valid_alloc3 : cs:circGCState -> init:state -> bexp:BoolExp -> cs':circGCState ->
+  Lemma (requires (validGCState cs init /\ cs' = snd (circGCAlloc cs bexp)))
+	(ensures  (forall q. Set.mem q (vals cs.symtab) ==> 
+                     evalBexp q.ival init = evalBexp (BXor (BVar q.id, q.cval)) (evalCirc cs'.gates init)))
+let valid_alloc3 cs init bexp cs' =
+  let bexp' = substVar bexp (getSubs cs.symtab) in
+  let (ah, bit) = popMin cs.ah in
+  let (ah', _, _, gates) = compileBexp ah bit bexp' in
+  let q = { id = bit; 
+            ival = BFalse; 
+            cval = bexp' } 
+  in
+  let init' = evalCirc cs'.gates init in
+    compile_mods ah bit bexp'
+
+val valid_alloc : cs:circGCState -> init:state -> bexp:BoolExp ->
+  Lemma (requires (validGCState cs init))
+	(ensures  (validGCState (snd (circGCAlloc cs bexp)) init))
+let valid_alloc cs init bexp =
+  let bexp' = substVar bexp (getSubs cs.symtab) in
+  let (ah, bit) = popMin cs.ah in
+  let (ah', _, _, gates) = compileBexp ah bit bexp' in
+  let q = { id = bit; 
+            ival = BFalse; 
+            cval = bexp' } 
+  in
+  let cs' = snd (circGCAlloc cs bexp) in
+  let init' = evalCirc cs'.gates init in
+  let zeroHeap_pres = admitP(zeroHeap init' ah')(*
+    //------------ 
+    pop_proper_subset cs.ah;
+    zeroHeap_subset (evalCirc cs.gates init) cs.ah ah;
+    compile_decreases_heap ah bit bexp';
+    zeroHeap_subset (evalCirc cs.gates init) ah cs'.ah;
+    //------------
+    subst_subset_active cs bexp;
+    disjoint_subset (elts ah) (elts cs.ah) (ids cs.symtab);
+    disjoint_subset (vars bexp') (ids cs.symtab) (elts ah);
+    compile_partition ah bit bexp';
+    zeroHeap_st_impl (evalCirc cs.gates init) cs'.ah gates*)
+  in
+  let disjoint_pres = //admitP(disjoint (ids cs'.symtab) (elts cs'.ah))
+    pop_proper_subset cs.ah;
+    compile_decreases_heap ah bit bexp'
+  in
+  let cleanup_pres =
+    //admitP(forall q. Set.mem q (vals cs.symtab) ==> 
+    //                      evalBexp q.ival init = evalBexp (BXor (BVar q.id, q.cval)) init')
+    compile_mods ah bit bexp'
+  in
+  let alloc_correct : u:unit{evalBexp q.ival init = evalBexp (BXor (BVar q.id, q.cval)) init'} =(*
+    pop_proper_subset cs.ah;
+    zeroHeap_subset (evalCirc cs.gates init) cs.ah ah;
+    //------------
+    subst_subset_active cs bexp;
+    disjoint_subset (elts ah) (elts cs.ah) (ids cs.symtab);
+    disjoint_subset (vars bexp') (ids cs.symtab) (elts ah);
+    //------------
+    compile_bexp_correct ah bit bexp' (evalCirc cs.gates init);
+    eval_mod (evalCirc cs.gates init) gates;
+    eval_state_swap (BXor (BVar q.id, q.cval)) (evalCirc cs.gates init) init';*)
+    admitP(b2t(evalBexp q.ival init = evalBexp (BXor (BVar q.id, q.cval)) init'))
+  in
+    ()
+
+type circ_equiv (st:boolState) (cs:circGCState) (init:state) =
+  validGCState cs init /\ fst st = cs.top /\ (forall i. boolEval st init i = circGCEval cs init i)
